add some docs

TypedAssembly/SystemF.lean
@@ -1,9 +1,6 @@
-import «TypedAssembly».Util 
 
-import Std.Data.List.Basic
-import Lean.Data.AssocList
-open Lean (AssocList)
-
+/-- A TCtx is essentally a Nat, representing the size of our
+    typing context -/
 inductive TCtx where
   | nil : TCtx
   | more : TCtx → TCtx
@@ -16,6 +13,7 @@ end TCtx
 
 open TCtx
 
+/-- A TypVar is essentially a Fin n, i.e., a pointer inside a Nat -/
 inductive TypVar : TCtx → Type where
   | here : TypVar ⊹Δ
   | there : TypVar Δ → TypVar ⊹Δ
@@ -31,11 +29,12 @@ inductive Typ : TCtx → Type where
   | var : Δ✓ → Typ Δ
   | int : Typ Δ
   | arrow : Typ Δ → Typ Δ → Typ Δ
+  | prod : Typ Δ → Typ Δ → Typ Δ
   | for_all : Typ ⊹Δ → Typ Δ
   deriving BEq, DecidableEq, Repr
 
 namespace Typ
-  postfix:max " ⊢⋆ " => Typ
+  postfix:90 " ⊢⋆ " => Typ
 
   declare_syntax_cat typvar
   syntax num : typvar
@@ -48,12 +47,14 @@ namespace Typ
 
   macro "♯ " n:term:90 : term => `(Typ.var (by get_elem $n))
 
-  def _x : Typ ⊹⊹⊹∅⋆ := ♯2
-  #eval _x
+  example :
+    Typ.var (TypVar.there (TypVar.there (TypVar.here))) = (♯2 : Typ ⊹⊹⊹∅⋆) := rfl 
 
   declare_syntax_cat typ
+  syntax "!" term:max : typ
   syntax:10 "∀. " typ : typ
   syntax:50 typ (" → " <|> " -> ") typ : typ
+  syntax:50 typ " × " typ : typ
   syntax:90 "♯" num : typ
   syntax " int " : typ
   syntax " ⋆⟪ " typ " ⟫ " : term
@@ -61,57 +62,103 @@ namespace Typ
   syntax " ( " typ " ) " : typ
   
   macro_rules 
+  | `( ⋆⟪ !$t ⟫) => `($t)
   | `( ⋆⟪ int ⟫ ) => `(Typ.int)
   | `( ⋆⟪ ♯$n ⟫ ) => `(♯$n)
   | `( ⋆⟪ $t₁:typ → $t₂:typ ⟫ ) => `(Typ.arrow ⋆⟪ $t₁ ⟫ ⋆⟪ $t₂ ⟫)
+  | `( ⋆⟪ $t₁:typ × $t₂:typ ⟫ ) => `(Typ.prod ⋆⟪ $t₁ ⟫ ⋆⟪ $t₂ ⟫)
   | `( ⋆⟪ ∀. $t:typ ⟫) => `(Typ.for_all ⋆⟪ $t ⟫)
   | `( ⋆⟪ ( $t )  ⟫ ) => `(⋆⟪ $t ⟫)
+
+  def polyidty : ∅⋆ ⊢⋆ := ⋆⟪ ∀. ♯0 → ♯0 ⟫
 end Typ
+open Typ
 
-def polyidty : Typ ∅⋆ := ⋆⟪ ∀. ♯0 → ♯0 ⟫
-#eval polyidty
 
+/-- A Ren⋆ Δ₁ Δ₂ is a funciton that takes a typ variable and moves it
+    from the first typing context to the second -/
 @[reducible]
-def Ren c₁ c₂ :=  c₁✓ → c₂✓
+def Rent Δ₁ Δ₂ := Δ₁✓ → Δ₂✓
 
+/-- lift⋆ takes a Ren⋆ and returns a different Ren⋆ that operates in a typing context
+    where the meaning of the first typvar is unaffected but all later typ variable
+    are shifted by 1 position -/
 @[reducible]
-def lift {c₁ c₂} : Ren c₁ c₂ → Ren ⊹c₁ ⊹c₂ 
+def liftt {Δ₁ Δ₂} : Rent Δ₁ Δ₂ → Rent ⊹Δ₁ ⊹Δ₂ 
   | _, .here => .here
   | r, .there a => .there (r a)
 
+/-- ren⋆ takes a Ren⋆ and a typ and moves all the typ variables in that typ to the
+    new context -/
 @[reducible]
-def ren {c₁ c₂} : Ren c₁ c₂ → c₁⊢⋆ → c₂⊢⋆
+def rent {Δ₁ Δ₂} : Rent Δ₁ Δ₂ → Δ₁⊢⋆ → Δ₂⊢⋆
   | _, .int => .int
   | r, .var a => .var (r a)
-  | r, .arrow a b => .arrow (ren r a) (ren r b)
-  | r, .for_all b => .for_all (ren (lift r) b)
+  | r, .arrow a b => .arrow (rent r a) (rent r b)
+  | r, .prod a b => .prod (rent r a) (rent r b)
+  | r, .for_all b => .for_all (rent (liftt r) b)
 
+/-- weaken⋆ shifts over all typ variables in a variable by 1 position,
+    e.g. ⋆⟪ ♯0 → ♯0 ⟫ : ⊹∅⋆ ⊢⋆ becomes ⋆⟪ ♯1 → ♯1 ⟫ : ⊹⊹∅⋆ ⊢⋆ -/
 @[reducible]
-def weaken {c} : c⊢⋆ → (⊹c)⊢⋆ := ren TypVar.there
+def weakent {c} : c⊢⋆ → (⊹c)⊢⋆ := rent TypVar.there
 
-@[reducible]
-def Subs c₁ c₂ := c₁✓ → c₂⊢⋆
+/-- A Subs⋆ Δ₁ Δ₂ is a function that takes a typ variable and returns 
+    a typ (in a possibly modified context) that should be in its place -/
+def Subst Δ₁ Δ₂ := Δ₁✓ → Δ₂⊢⋆
 
-@[reducible]
-def lifts {c₁ c₂} : Subs c₁ c₂ → Subs ⊹c₁ ⊹c₂
+/-- lifts⋆ takes a Subs⋆ and returns a different Subs⋆ that operates in a typing context where
+    the meaning of the first typevar is unaffected but all later type variables are shifted by 1 position -/
+@[reducible, simp]
+def liftst {Δ₁ Δ₂} : Subst Δ₁ Δ₂ → Subst ⊹Δ₁ ⊹Δ₂
   | _, .here => .var .here
-  | s, .there a => weaken (s a)
+  | s, .there a => weakent (s a)
 
-@[reducible]
-def subs {c₁ c₂} : Subs c₁ c₂ → c₁⊢⋆ → c₂⊢⋆
+/-- subs⋆ takes a Subs⋆ and a type and replaces the relevant type variable with that type, 
+    returning a new type (in a possibly modified context) -/
+@[reducible, simp]
+def subst {Δ₁ Δ₂} : Subst Δ₁ Δ₂ → Δ₁⊢⋆ → Δ₂⊢⋆
   | _, .int => .int
   | s, .var a => s a
-  | s, .arrow a b => .arrow (subs s a) (subs s b)
-  | s, .for_all b => .for_all (subs (lifts s) b)
+  | s, .arrow a b => .arrow (subst s a) (subst s b)
+  | s, .prod a b => .prod (subst s a) (subst s b)
+  | s, .for_all b => .for_all (subst (liftst s) b)
 
+/-- inst⋆ takes a Subs⋆ and a type and returns a Subs⋆ that
+    replaces the position 0 type variables with that type, otherwise 
+    it applies the first Subs⋆ to a shifted down typevar -/
 @[reducible]
-def inst {c₁ c₂} : Subs c₁ c₂ → c₂⊢⋆ → Subs ⊹c₁ c₂ 
+def instt {Δ₁ Δ₂} : Subst Δ₁ Δ₂ → Δ₂⊢⋆ → Subst ⊹Δ₁ Δ₂ 
   | _, t, TypVar.here => t
   | s, _, TypVar.there a => s a
 
-macro b:term:80 "[" a:term:80 "]⋆" : term =>  `(subs (inst .var $a) $b)
+macro b:term:80 "[" a:term:80 "]⋆" : term =>
+  -- .var is indeed the identity Subs⋆, so this replaces ♯0
+  -- with $a, otherwise makes ♯n ♯(n-1)
+  `(subst (instt .var $a) $b) 
 
-#eval (⋆⟪ ♯0 → ♯0 ⟫ : @Typ ⊹∅⋆ )[.int]⋆
+theorem «.var is identity subst» : ∀ (t : Δ⊢⋆), subst .var t = t := by
+  intros t
+  induction t <;>
+    try rfl 
+  case arrow =>
+    simp
+    constructor <;> assumption
+  case prod =>
+    simp
+    constructor <;> assumption
+
+  case for_all Δ' t' t_ih =>
+    simp only [subst]
+    congr
+    have : @liftst Δ' Δ' Typ.var = Typ.var := by
+          simp
+          funext x 
+          cases x <;> rfl
+    rw [this]
+    assumption
+
+example : ⋆⟪ ♯0 → ♯0 ⟫[.int]⋆ = (⋆⟪ int → int ⟫ : Typ ∅⋆) := rfl
 
 inductive Prim where
   | plus
@@ -121,11 +168,11 @@ inductive Prim where
 
 inductive Ctx : TCtx → Type where
   | nil : Ctx Δ
-  | cons_kind : Ctx Δ → Ctx ⊹Δ
-  | cons_typ : Ctx Δ → c⊢⋆ → Ctx Δ
+  | snoc_kind : Ctx Δ → Ctx ⊹Δ
+  | snoc_typ : Ctx Δ → c⊢⋆ → Ctx Δ
 
 namespace Ctx
-  infixl:50 " ‘ " => Ctx.cons_typ
+  infixl:50 " ‘ " => Ctx.snoc_typ
   notation "∅" => Ctx.nil
 end Ctx
 open Ctx
@@ -133,7 +180,7 @@ open Ctx
 inductive Lookup : Ctx Δ → Δ⊢⋆ → Type where
 | here : Lookup (Γ ‘ t) t
 | there : Lookup Γ t → Lookup (Γ ‘ t') t
-| move : Lookup Γ t → Lookup Γ.cons_kind (weaken t)
+| move : Lookup Γ t → Lookup Γ.snoc_kind (weakent t)
 deriving Repr
 
 namespace Lookup
@@ -141,21 +188,25 @@ namespace Lookup
 end Lookup
 open Lookup
 
-inductive Term : {Δ : TCtx} → Ctx Δ → Typ Δ → Type where
-  | int {Γ : Ctx Δ} : Int → Term Γ .int
-  | var {Γ : Ctx Δ} {t : Δ⊢⋆} : Γ ∋ t → Term Γ t
-  | fix {Γ : Ctx Δ} {t₁ t₂ : Δ⊢⋆} : Term (Γ ‘ t₁ ‘ (.arrow t₁ t₂)) t₂ → Term Γ (.arrow t₁ t₂)
-  | app {Γ : Ctx Δ} {t₁ t₂ : Δ⊢⋆} : Term Γ (.arrow t₁ t₂) → Term Γ t₁ → Term Γ t₂
+inductive Term : (Δ : TCtx) → Ctx Δ → Typ Δ → Type where
+  | int  {Γ : Ctx Δ} : Int → Term Δ Γ .int
+  | var  {Γ : Ctx Δ} {t : Δ⊢⋆} : Γ ∋ t → Term Δ Γ t
 
-  | Λ   {Γ : Ctx Δ} {t : (⊹Δ)⊢⋆} : Term Γ.cons_kind t → Term Γ (.for_all t)
-  | sub {Γ : Ctx Δ} {t' : (⊹Δ)⊢⋆} : Term Γ (.for_all t') → (t : Δ⊢⋆) → Term Γ (t'[t]⋆)
+  | fix  {Γ : Ctx Δ} {t₁ t₂ : Δ⊢⋆} : Term Δ (Γ ‘ t₁ ‘ ⋆⟪ !t₁ → !t₂ ⟫) t₂ → Term Δ Γ ⋆⟪ !t₁ → !t₂ ⟫
+  | app  {Γ : Ctx Δ} {t₁ t₂ : Δ⊢⋆} : Term Δ Γ ⋆⟪ !t₁ → !t₂ ⟫ → Term Δ Γ t₁ → Term Δ Γ t₂
 
-  | prim  {Γ : Ctx Δ} : Term Γ .int → Prim → Term Γ .int → Term Γ .int
-  | if0 {Γ : Ctx Δ} {t : Δ⊢⋆}: Term Γ .int → Term Γ t → Term Γ t → Term Γ t
+  | Λ    {Γ : Ctx Δ} {t : (⊹Δ)⊢⋆} : Term ⊹Δ Γ.snoc_kind t → Term Δ Γ ⋆⟪ ∀. !t ⟫
+  | sub  {Γ : Ctx Δ} {t' : (⊹Δ)⊢⋆} : Term Δ Γ ⋆⟪ ∀. !t' ⟫ → (t : Δ⊢⋆) → Term Δ Γ (t'[t]⋆)
+
+  | prim {Γ : Ctx Δ} : Term Δ Γ .int → Prim → Term Δ Γ .int → Term Δ Γ .int
+  | pair {Γ : Ctx Δ} : Term Δ Γ t₁ → Term Δ Γ t₂ → Term Δ Γ ⋆⟪ !t₁ × !t₂ ⟫
+  | fst {Γ : Ctx Δ} : Term Δ Γ ⋆⟪ !t₁ × !t₂ ⟫ → Term Δ Γ t₁
+  | snd {Γ : Ctx Δ} : Term Δ Γ ⋆⟪ !t₁ × !t₂ ⟫ → Term Δ Γ t₂
+  | if0  {Γ : Ctx Δ} {t : Δ⊢⋆}: Term Δ Γ .int → Term Δ Γ t → Term Δ Γ t → Term Δ Γ t
   deriving Repr
 
 namespace Term 
-  infix:40 " ⊢ " => Term
+  notation:10 Δ " ∣ " Γ " ⊢ " t => Term Δ Γ t
 
   syntax "get_elem'" (ppSpace term) : tactic
   macro_rules | `(tactic| get_elem' $n) => match n.1.toNat with
@@ -164,10 +215,11 @@ namespace Term
 
   macro "# " n:term:90 : term => `(Term.var (by get_elem' $n))
 
-  def _x : @Term ∅⋆ (∅ ‘ (@Typ.int ∅⋆) ‘ (@Typ.int ∅⋆)) .int := #1
-  #eval _x
+  example : ∅⋆ ∣ (∅ ‘ (@Typ.arrow ∅⋆ .int .int) ‘ (@Typ.int ∅⋆)) ⊢ ⋆⟪ int ⟫ := #0
+  example : ∅⋆ ∣ (∅ ‘ (@Typ.arrow ∅⋆ .int .int) ‘ (@Typ.int ∅⋆)) ⊢ ⋆⟪ int → int ⟫ := #1
   
   declare_syntax_cat trm
+  syntax "!" term:max : trm
   syntax num : trm 
   syntax "#" num : trm
   syntax " λ. " trm : trm
@@ -177,13 +229,17 @@ namespace Term
   syntax:20 trm:20 " + " trm:21 : trm
   syntax:20 trm:20 " - " trm:21 : trm
   syntax:30 trm:30 " * " trm:31 : trm
+  syntax " ( " trm ", " trm " ) " : trm
+  syntax "π₁" trm : trm
+  syntax "π₂" trm : trm
   syntax "if0 " trm " then " trm " else " trm " end " : trm
+  syntax "if0 " " ( " trm " , " trm " , " trm " ) " : trm
 
   syntax " ( " trm " ) " : trm
-
   syntax " ⟪ " trm " ⟫" : term
 
   macro_rules
+    | `( ⟪ !$t ⟫) => `($t)
     | `( ⟪ $i:num ⟫ ) => `(Term.int $i)
     | `( ⟪ #$i:num ⟫ ) => `(#$i)
     | `( ⟪ λ. $e ⟫ ) => `(Term.fix ⟪ $e ⟫)
@@ -193,36 +249,87 @@ namespace Term
     | `( ⟪ $e₁ + $e₂ ⟫ ) => `(Term.prim ⟪ $e₁ ⟫ Prim.plus ⟪ $e₂ ⟫ )
     | `( ⟪ $e₁ - $e₂ ⟫ ) => `(Term.prim ⟪ $e₁ ⟫ Prim.minus ⟪ $e₂ ⟫ )
     | `( ⟪ $e₁ * $e₂ ⟫ ) => `(Term.prim ⟪ $e₁ ⟫ Prim.times ⟪$e₂ ⟫ )
+    | `( ⟪ ($e₁, $e₂) ⟫) => `(Term.pair ⟪ $e₁ ⟫ ⟪$e₂ ⟫ )
+    | `( ⟪ π₁ $e ⟫) => `(Term.fst ⟪ $e ⟫ )
+    | `( ⟪ π₂ $e ⟫) => `(Term.snd ⟪ $e ⟫ )
     | `( ⟪ if0 $e₁ then $e₂ else $e₃ end ⟫ ) => `(Term.if0 ⟪ $e₁ ⟫ ⟪ $e₂ ⟫ ⟪ $e₃ ⟫ )
+    | `( ⟪ if0 ($e₁, $e₂, $e₃) ⟫ ) => `(Term.if0 ⟪ $e₁ ⟫ ⟪ $e₂ ⟫ ⟪ $e₃ ⟫ )
 
-    | `( ⟪ ( $e ) ⟫ ) => `( ⟪ $e ⟫ )
+    | `( ⟪ ( $e ) ⟫ ) => `( ⟪ $e ⟫ ) 
 end Term
 open Term
 
-def fact : @Term ∅⋆ ∅ ⋆⟪ int → int ⟫ :=
-  Term.fix (Term.if0 (.var (.there .here))
+def fact : ∅⋆ ∣ ∅ ⊢ ⋆⟪ int → int ⟫ :=
+  Term.fix (.if0 (.var (.there .here))
             (.int 1)
             (.prim (.var (.there .here)) .times (.app (.var .here) (Term.prim (.var (.there .here)) .minus (.int 1)))))
+#eval fact
 
-def fact' Δ Γ : @Term Δ Γ ⋆⟪ int → int ⟫ := 
+def fact' : ∅⋆ ∣ ∅ ⊢ ⋆⟪ int → int ⟫ := 
   ⟪ λ. if0 #1 then
          1
        else
          #1 * (#0 (#1 - 1))
        end ⟫
-           
 
-#eval fact
+#eval fact'
 
-def sixfact := Term.app fact (.int 6)
-#eval sixfact
+theorem fact_eq_fact' : fact = fact' := rfl
 
-def freeid : @Term ⊹∅⋆ ∅.cons_kind ⋆⟪ ♯0 → ♯0 ⟫ :=
+def sixfact := ⟪ !fact 6 ⟫
+
+def freeid : ⊹∅⋆ ∣ ∅.snoc_kind ⊢ ⋆⟪ ♯0 → ♯0 ⟫ :=
  ⟪ λ. #1 ⟫
 
-def intid : @Term ∅⋆ ∅ ⋆⟪ int → int ⟫ := 
-  Term.sub (Term.Λ freeid) .int
-
+def intid := ⟪ (Λ. !freeid)[int] ⟫
 #eval intid
 
+@[reducible]
+def Ren : ∀ {Δ₁ Δ₂}, Ctx Δ₁ → Ctx Δ₂ → Rent Δ₁ Δ₂ → Type := 
+  fun Γ₁ Γ₂ rt => {a : _ ⊢⋆} → Γ₁ ∋ a → Γ₂ ∋ rent rt a
 
+
+@[reducible]
+def lift : ∀ {Δ₁ Δ₂ Γ₁ Γ₂} {rt : Rent Δ₁ Δ₂}, 
+          Ren Γ₁ Γ₂ rt → {b : Δ₁ ⊢⋆} → Ren (Γ₁ ‘ b) (Γ₂ ‘ rent rt b) rt := 
+    fun r _ b x => 
+      match x with
+      | .here => .here
+      | .there x' => .there (r x')
+
+def convninf {Δ Γ} {a₁ a₂ : Δ ⊢⋆} :  
+              a₁ = a₂ → Γ ∋ a₁ → Γ ∋ a₂
+      | rfl, x => x
+
+@[reducible]
+def tlift : ∀ {Δ₁ Δ₂ Γ₁ Γ₂} {rt : Rent Δ₁ Δ₂}, 
+            Ren Γ₁ Γ₂ rt → {b : Δ₁ ⊢⋆} → Ren Γ₁.snoc_kind Γ₂.snoc_kind (liftt rt) := by
+    intros Δ₁ Δ₂ Γ₁ Γ₂ rt r b a v
+    cases v with
+    | move v => admit
+
+abbrev interp : Prim → (Int → Int → Int)
+  | .plus => Int.add
+  | .minus => Int.sub
+  | .times => Int.mul
+
+inductive Step {Δ Γ} : (Δ ∣ Γ ⊢ t) → (Δ ∣ Γ ⊢ t) → Prop
+  | prim_exec  : Step (.prim (.int n₁) p (.int n₂)) (.int (interp p n₁ n₂))
+  | prim_left  : Step a a' → Step (.prim a p b) (.prim a' p b)
+  | prim_right : Step b b' → Step (.prim (.int n) p b) (.prim (.int n) p b')
+
+  | fst_exec   : Step ⟪ π₁(!e, !_) ⟫ e
+  | fst_steps  : Step e e' →  Step (.fst e) (.fst e')
+
+  | snd_exec   : Step ⟪ π₂(!_, !e) ⟫ e
+  | snd_steps  : Step e e' →  Step (.snd e) (.snd e')
+
+  | if0_exec   : Step ⟪ if0 0 then !b else !c end ⟫ b
+  | ifn0_exec  : n ≠ 0 → Step ⟪ if0 !(.int n) then !b else !c end ⟫ c
+  | if_steps   : Step a a' → Step ⟪ if0 !a then !b else !c end ⟫ ⟪ if0 !a' then !b else !c end ⟫
+
+inductive MultiStep {Δ Γ t} : (Δ ∣ Γ ⊢ t) → (Δ ∣ Γ ⊢ t) → Prop 
+  | refl {a} : MultiStep a a
+  | step {a b c} : Step a b → MultiStep b c → MultiStep a c
+
+theorem «1+1 -->* 2» : MultiStep (Δ := ∅⋆) (Γ := ∅) ⟪ if0 0 then 1 + 1 else 5 end ⟫ ⟪ 2 ⟫ := by repeat constructor
